ratchet/corpus/235-lambda-capture-reassigned-same-type.rb
@@ -1,0 +1,4 @@
+x = 1
+f = lambda { x }
+x = 2
+f.call + 1
